src/Generic.v
@@ -1,0 +1,35 @@
+Require Import List.
+Require Import ExtLib.Data.Vector.
+
+Set Implicit Arguments.
+Set Strict Implicit.
+
+Section quant.
+  Variable T : Type.
+
+  Fixpoint quant (n : nat) : Type :=
+    match n with
+      | 0 => T
+      | S n => T -> quant n
+    end.
+
+  Fixpoint qapply (n : nat) (ls : list T) : quant n -> option T :=
+    match n as n , ls return quant n -> option T with
+      | 0 , nil => fun t => Some t
+      | S n , l :: ls => fun f => @qapply n ls (f l)
+      | _ , _ => fun _ => None
+    end.
+
+  Fixpoint qapply_v (n : nat) : vector T n -> quant n -> T :=
+    match n as n return vector T n -> quant n -> T with
+      | 0 => fun _ x => x
+      | S n => fun args x => qapply_v n (snd args) (x (fst args))
+    end.
+
+  Fixpoint parametric (n : nat) (acc : list T) (k : list T -> Type) : Type :=
+    match n with
+      | 0 => k acc
+      | S n => forall T : T, parametric n (T :: acc) k
+    end.
+
+End quant.
