src/TypesExtDemo.v
@@ -1,0 +1,151 @@
+Require Import List.
+Require Import ExtLib.Core.RelDec.
+Require Import ExtLib.Core.Type.
+Require Import MirrorCore.TypesExt.
+
+Module example.
+
+  Inductive my_type : Type :=
+  | List : my_type -> my_type
+  | Nat : my_type
+  | Arr : my_type -> my_type -> my_type
+  | Var : nat -> my_type.
+
+  Fixpoint my_typeD (ts : list Type) (t : my_type) : Type :=
+    match t with
+      | List t => list (my_typeD ts t)
+      | Nat => nat
+      | Arr d r => my_typeD ts d -> my_typeD ts r
+      | Var v => match nth_error ts v with
+                   | Some T => T
+                   | None => Empty_set
+                 end
+    end.
+
+  Fixpoint my_type_eq (a b : my_type) {struct a} : option (a = b).
+  refine (
+    match a , b with
+      | Nat , Nat => Some eq_refl
+      | List a , List b =>
+        match my_type_eq a b with
+          | Some pf => Some _
+          | None => None
+        end
+      | Arr ad ar , Arr bd br => 
+        match my_type_eq ad bd , my_type_eq ar br with
+          | Some _ , Some _ => Some _
+          | _ , _ => None
+        end
+      | Var x , Var y =>
+        match EqNat.beq_nat x y as z return z = EqNat.beq_nat x y -> option (Var x = Var y) with
+          | true => fun pf => Some _
+          | false => fun _ => None
+        end eq_refl 
+      | _ , _ => None
+    end); subst; try reflexivity.
+  rewrite (EqNat.beq_nat_eq _ _ pf). reflexivity.
+  Defined.
+  
+  Definition my_type_cast ts (a b : my_type) : option (my_typeD ts a -> my_typeD ts b) :=
+    match my_type_eq a b with
+      | None => None
+      | Some pf => Some match pf in _ = a' return (my_typeD ts a -> my_typeD ts a') with
+                          | eq_refl => fun x => x
+                        end
+    end.
+(* This requires well-founded recursion, e.g. recursion on the sum of the heights
+  Fixpoint my_type_cast (a b : my_type) {struct b} : option (my_typeD a -> my_typeD b) :=
+    match a as a , b as b return option (my_typeD a -> my_typeD b) with
+      | Nat , Nat => Some (fun x => x)
+      | List a , List b => 
+        match my_type_cast a b with
+          | None => None
+          | Some f => Some (map f)
+        end
+      | Arr ad ar , Arr bd br =>
+        match my_type_cast bd ad , my_type_cast ar br with
+          | Some dcast , Some rcast =>
+            Some (fun f => (fun x => rcast (f (dcast x))))
+          | _ , _ => None
+        end
+      | _ , _ => None
+    end.
+*)
+
+  Fixpoint my_type_eqb ts (a : my_type) : my_typeD ts a -> my_typeD ts a -> option bool :=
+    match a as a return my_typeD ts a -> my_typeD ts a -> option bool with 
+      | Nat => fun x y => Some (x ?[ eq ] y)
+      | List a =>
+        let C := my_type_eqb ts a in
+        fix cmp (x y : list (my_typeD ts a)) {struct x} : option bool :=
+          match x , y with 
+            | nil , nil => Some true
+            | x :: xs , y :: ys => 
+              match C x y with
+                | Some false => Some false
+                | None => match cmp xs ys with
+                            | Some false => Some false
+                            | _ => None
+                          end
+                | Some true => cmp xs ys
+              end
+            | _ , _ => Some false
+          end
+        | Arr _ _ => fun _ _ => None
+        | Var _ => fun _ _ => None
+    end.
+
+  Require Import ExtLib.Data.Nat.
+  Require Import ExtLib.Data.List.
+  Require Import ExtLib.Data.Fun.
+
+  Instance RType_my_type : RType my_typeD :=
+  { typ_cast := my_type_cast
+  ; eqb := my_type_eqb
+  ; typeFor := fun ts => fix typeFor t : type (my_typeD ts t) :=
+               match t as t return type (my_typeD ts t) with
+                 | Nat => type_nat
+                 | List t => @type_list _ (typeFor t)
+                 | Arr a b => type_Fun (typeFor a) (typeFor b)
+                 | Var v => type_libniz _
+               end
+  ; instantiate_typ := fun _ x => x
+  ; type_of_apply := fun y x => match x with
+                                  | nil => Some y
+                                  | _ => None
+                                end
+  ; type_apply := fun _ _ _ _ _ => None
+  }.
+
+  Instance TypInstance_nat : @TypInstance0 _ my_typeD nat :=
+  { ctor0 := Nat
+  ; ctor0_iso := fun _ => {| into := fun x => x ; outof := fun x => x |}
+  ; ctor0_match := fun ts R caseNat caseElse t =>
+                    match t as t return R t (my_typeD ts t) with
+                      | Nat => caseNat tt
+                      | _ => caseElse _
+                    end
+  }.
+
+  Instance TypInstance1_list : @TypInstance1 _ my_typeD list :=
+  { ctor1 := List
+  ; ctor1_iso := fun _ _ => {| into := fun x => x ; outof := fun x => x |}
+  ; ctor1_match := fun ts R caseList caseElse t =>
+      match t as t return R t (my_typeD ts t) with
+        | List t => caseList t
+        | _ => caseElse _
+      end
+  }.
+
+  Definition Fun D R : Type := D -> R.
+  Instance TypInstance2_arr : @TypInstance2 _ my_typeD Fun :=
+  { ctor2 := Arr
+  ; ctor2_iso := fun _ _ _ => {| into := fun x => x ; outof := fun x => x |}
+  ; ctor2_match := fun ts R caseArr caseElse t =>
+      match t as t return R t (my_typeD ts t) with
+        | Arr t1 t2 => caseArr t1 t2
+        | _ => caseElse _
+      end
+  }.
+
+End example.
